Makefile
@@ -1,0 +1,3 @@
+all: 
+	coqc specification/Dynamics.v
+	coqc specification/Statics.v
